% preamble
\documentclass{article}

\title{Cross-entropy loss with regularization and its gradients}
\author{}
\date{\vspace{-5ex}}

% packages
\usepackage{amsmath}

% main document
\begin{document}
  \maketitle
  
  Notation:\\
  n - number of train examples (batch\_size);\\
  d - number of dimensions of an example;\\
  c - number of classes (10 classes for CIFAR-10);\\
  y - labels of correct classes ($y_{i}$ - the correct label for the ith example);

  \begin{align*}
  L &= \frac{1}{n} \sum_{i}^{n} L_{i} 
       + \lambda * \sum_{j}^{d} \sum_{k}^{c} W_{j,k}^{2}\\
  L_{i} &= -\ln{p_{y_{i}}} [cross-entropy]\\
  p_{k} &= \frac {e^{z_{y_{k}}}}{\sum_{j}^{c} e^{z_{j}}} [softmax]\\
  z_{j} &= X * W_{j} [score-for-example-X-to-belong-to-class-j]\\
  \frac {\partial L_{i}}{\partial p_{i}} &= -\frac {1}{p_{i}}\\
  \frac {\partial p_{k}}{\partial z_{y_{k}}} &= 
        \frac {e^{z_{y_{k}}}\sum_{j}^{c} e^{z_{j}} - e^{z_{y_{k}}}e^{z_{y_{k}}}}
              {(\sum_{j}^{c} e^{z_{j}})^2} 
      = \frac {e^{z_{y_{k}}}}{\sum_{j}^{c} e^{z_{j}}}
        -
        \frac {e^{z_{y_{k}}}}{\sum_{j}^{c} e^{z_{j}}}
        \frac {e^{z_{y_{k}}}}{\sum_{j}^{c} e^{z_{j}}}
      = p_{k} - p_{k}^2
      = p_{k}(1 - p_{k})\\
  \frac {\partial p_{k}}{\partial z_{l}} &= 
        -\frac {e^{z_{y_{k}}}e^{z_{l}}}
               {(\sum_{j}^{c} e^{z_{j}})^2}
       = -\frac {e^{z_{y_{k}}}}{\sum_{j}^{c} e^{z_{j}}}
          \frac {e^{z_{l}}}{\sum_{j}^{c} e^{z_{j}}} 
       = -p_{k}p_{l} [l \neq y_{k}]\\
  \frac {\partial z_{j}}{\partial w_{j}} &= X\\
  \frac {\partial L_{i}}{\partial w_{y_{i}}} &=
         \frac {\partial L_{i}}{\partial p_{i}}
         \frac {\partial p_{i}}{\partial z_{y_{i}}}
         \frac {\partial z_{y_{i}}}{\partial w_{y_{i}}}
      = -\frac {1}{p_{i}}{p_{i}}(1 - p_{i})X
      = (p_{i} - 1)X [y_{i}, chain- rule]\\
  \frac {\partial L_{i}}{\partial w_{j}} &=
         \frac {\partial L_{i}}{\partial p_{i}}
         \frac {\partial p_{i}}{\partial z_{j}}
         \frac {\partial z_{j}}{\partial w_{j}}
      = -\frac {1}{p_{i}}(-p_{i}p_{j})X
      = p_{j}X [j \neq y_{i}, chain- rule]
  \end{align*}

\end{document}